coq/src/Concordium_Impls_template.v
@@ -5,6 +5,453 @@ Import List.ListNotations.
 Open Scope Z_scope.
 Open Scope bool_scope.
 Open Scope hacspec_scope.
+Inductive log_error_t :=
+| Full : log_error_t
+| Malformed : log_error_t.
+
+Definition eqb_log_error_t (x y : log_error_t) : bool :=
+match x with
+   | Full => match y with | Full=> true | _ => false end
+   | Malformed => match y with | Malformed=> true | _ => false end
+   end.
+
+Definition eqb_leibniz_log_error_t (x y : log_error_t) : eqb_log_error_t x y = true <-> x = y.
+Proof. split. intros; destruct x ; destruct y ; try (f_equal ; apply eqb_leibniz) ; easy. intros ; subst ; destruct y ; try reflexivity ; try (apply eqb_refl). Qed.
+
+Instance eq_dec_log_error_t : EqDec (log_error_t) :=
+Build_EqDec (log_error_t) (eqb_log_error_t) (eqb_leibniz_log_error_t).
+
+
+Definition load_state_hacspec
+  (buf_0 : public_byte_seq)
+  (offset_1 : int32)
+  : (public_byte_seq × int32) :=
+  (buf_0, @repr WORDSIZE32 1).
+
+Definition write_state_hacspec
+  (buf_2 : public_byte_seq)
+  (offset_3 : int32)
+  : (public_byte_seq × int32) :=
+  (buf_2, @repr WORDSIZE32 1).
+
+Definition state_size_hacspec  : int32 :=
+  @repr WORDSIZE32 1.
+
+Definition resize_state_hacspec (new_size_4 : int32) : int32 :=
+  @repr WORDSIZE32 1.
+
+Definition get_parameter_section_hacspec
+  (buf_5 : public_byte_seq)
+  (offset_6 : int32)
+  : (public_byte_seq × int32) :=
+  (buf_5, @repr WORDSIZE32 1).
+
+Definition get_parameter_size_hacspec  : int32 :=
+  @repr WORDSIZE32 1.
+
+Definition get_slot_time_hacspec  : int64 :=
+  @repr WORDSIZE64 1.
+
+Definition get_policy_section_hacspec
+  (policy_bytes_7 : public_byte_seq)
+  (offset_8 : int32)
+  : (public_byte_seq × int32) :=
+  (policy_bytes_7, @repr WORDSIZE32 1).
+
+Definition get_init_origin_hacspec
+  (start_9 : public_byte_seq)
+  : public_byte_seq :=
+  start_9.
+
+Definition get_receive_invoker_hacspec
+  (start_10 : public_byte_seq)
+  : public_byte_seq :=
+  start_10.
+
+Definition get_receive_self_address_hacspec
+  (start_11 : public_byte_seq)
+  : public_byte_seq :=
+  start_11.
+
+Definition get_receive_self_balance_hacspec  : int64 :=
+  @repr WORDSIZE64 1.
+
+Definition get_receive_sender_hacspec
+  (start_12 : public_byte_seq)
+  : public_byte_seq :=
+  start_12.
+
+Definition get_receive_owner_hacspec
+  (start_13 : public_byte_seq)
+  : public_byte_seq :=
+  start_13.
+
+Definition log_event_hacspec
+  (start_14 : public_byte_seq)
+  : (public_byte_seq × int32) :=
+  (start_14, @repr WORDSIZE32 1).
+
+Definition accept_hacspec  : int32 :=
+  @repr WORDSIZE32 1.
+
+Definition simple_transfer_hacspec
+  (buf_15 : public_byte_seq)
+  (amount_16 : int64)
+  : int32 :=
+  @repr WORDSIZE32 1.
+
+Definition send_hacspec
+  (addr_index_17 : int64)
+  (addr_subindex_18 : int64)
+  (receive_name_19 : public_byte_seq)
+  (amount_20 : int64)
+  (parameter_21 : public_byte_seq)
+  : int32 :=
+  @repr WORDSIZE32 1.
+
+Definition combine_and_hacspec (l_22 : int32) (r_23 : int32) : int32 :=
+  @repr WORDSIZE32 1.
+
+Definition combine_or_hacspec (l_24 : int32) (r_25 : int32) : int32 :=
+  @repr WORDSIZE32 1.
+
+Require Import Hacspec.Lib.
+
+Notation "'reject_hacspec_t'" := (int32) : hacspec_scope.
+
+Definition reject_impl_deafult  : reject_hacspec_t :=
+  min_v.
+
+Definition new_reject_impl (x_26 : int32) : (option int32) :=
+  (if ((x_26) <.? (@repr WORDSIZE32 0)):bool then (@Some int32 (x_26)) else (
+      @None int32)).
+
+Definition reject_impl_convert_from_unit  : reject_hacspec_t :=
+  (min_v) .+ (@repr WORDSIZE32 1).
+
+Theorem ensures_reject_impl_convert_from_unit : forall result_27 ,
+@reject_impl_convert_from_unit  = result_27 ->
+~ (result_27 = @repr WORDSIZE32 0).
+Proof. Admitted.
+
+Definition reject_impl_convert_from_parse_error  : reject_hacspec_t :=
+  (min_v) .+ (@repr WORDSIZE32 2).
+
+Theorem ensures_reject_impl_convert_from_parse_error : forall result_27 ,
+@reject_impl_convert_from_parse_error  = result_27 ->
+~ (result_27 = @repr WORDSIZE32 0).
+Proof. Admitted.
+
+Definition reject_impl_from_log_error
+  (le_28 : log_error_t)
+  : reject_hacspec_t :=
+  match le_28 with
+  | Full => (min_v) .+ (@repr WORDSIZE32 3)
+  | Malformed => (min_v) .+ (@repr WORDSIZE32 4)
+  end.
+
+Theorem ensures_reject_impl_from_log_error : forall result_27 (
+  le_28 : log_error_t),
+@reject_impl_from_log_error le_28 = result_27 ->
+~ (result_27 = @repr WORDSIZE32 0).
+Proof. Admitted.
+
+Inductive new_contract_name_error_t :=
+| NewContractNameErrorMissingInitPrefix : new_contract_name_error_t
+| NewContractNameErrorTooLong : new_contract_name_error_t
+| NewContractNameErrorContainsDot : new_contract_name_error_t
+| NewContractNameErrorInvalidCharacters : new_contract_name_error_t.
+
+Definition reject_impl_from_new_contract_name_error
+  (nre_29 : new_contract_name_error_t)
+  : reject_hacspec_t :=
+  match nre_29 with
+  | NewContractNameErrorMissingInitPrefix => (min_v) .+ (@repr WORDSIZE32 5)
+  | NewContractNameErrorTooLong => (min_v) .+ (@repr WORDSIZE32 6)
+  | NewContractNameErrorContainsDot => (min_v) .+ (@repr WORDSIZE32 9)
+  | NewContractNameErrorInvalidCharacters => (min_v) .+ (@repr WORDSIZE32 10)
+  end.
+
+Theorem ensures_reject_impl_from_new_contract_name_error : forall result_27 (
+  nre_29 : new_contract_name_error_t),
+@reject_impl_from_new_contract_name_error nre_29 = result_27 ->
+~ (result_27 = @repr WORDSIZE32 0).
+Proof. Admitted.
+
+Inductive new_receive_name_error_t :=
+| NewReceiveNameErrorMissingDotSeparator : new_receive_name_error_t
+| NewReceiveNameErrorTooLong : new_receive_name_error_t
+| NewReceiveNameErrorInvalidCharacters : new_receive_name_error_t.
+
+Definition reject_impl_from_new_receive_name_error
+  (nre_30 : new_receive_name_error_t)
+  : reject_hacspec_t :=
+  match nre_30 with
+  | NewReceiveNameErrorMissingDotSeparator => (min_v) .+ (@repr WORDSIZE32 7)
+  | NewReceiveNameErrorTooLong => (min_v) .+ (@repr WORDSIZE32 8)
+  | NewReceiveNameErrorInvalidCharacters => (min_v) .+ (@repr WORDSIZE32 11)
+  end.
+
+Theorem ensures_reject_impl_from_new_receive_name_error : forall result_27 (
+  nre_30 : new_receive_name_error_t),
+@reject_impl_from_new_receive_name_error nre_30 = result_27 ->
+~ (result_27 = @repr WORDSIZE32 0).
+Proof. Admitted.
+
+Notation "'contract_state_hacspec_t'" := (int32) : hacspec_scope.
+
+Inductive seek_from_hacspec_t :=
+| Start : int64 -> seek_from_hacspec_t
+| End : int64 -> seek_from_hacspec_t
+| Current : int64 -> seek_from_hacspec_t.
+
+Notation "'uint32_option_t'" := ((option int32)) : hacspec_scope.
+
+Notation "'iint64_option_t'" := ((option int64)) : hacspec_scope.
+
+Definition contract_state_impl_seek
+  (current_position_31 : contract_state_hacspec_t)
+  (pos_32 : seek_from_hacspec_t)
+  : (result (contract_state_hacspec_t × int64) unit) :=
+  match pos_32 with
+  | Start offset_33 => @Ok (contract_state_hacspec_t × int64) unit ((
+      @cast _ uint32 _ (offset_33),
+      offset_33
+    ))
+  | End delta_34 => (if ((delta_34) >=.? (@repr WORDSIZE64 0)):bool then (
+      match pub_uint32_checked_add (current_position_31) (@cast _ uint32 _ (
+          delta_34)) with
+      | Some b_35 => @Ok (contract_state_hacspec_t × int64) unit ((
+          b_35,
+          @cast _ uint64 _ (delta_34)
+        ))
+      | None => @Err (contract_state_hacspec_t × int64) unit (tt)
+      end) else (match pub_int64_checked_abs (delta_34) with
+      | Some b_36 => @Ok (contract_state_hacspec_t × int64) unit ((
+          (@repr WORDSIZE32 4) .- (@cast _ uint32 _ (b_36)),
+          @cast _ uint64 _ ((@repr WORDSIZE32 4) .- (@cast _ uint32 _ (b_36)))
+        ))
+      | None => @Err (contract_state_hacspec_t × int64) unit (tt)
+      end))
+  | Current delta_37 => (if ((delta_37) >=.? (@repr WORDSIZE64 0)):bool then (
+      match pub_uint32_checked_add (current_position_31) (@cast _ uint32 _ (
+          delta_37)) with
+      | Some offset_38 => @Ok (contract_state_hacspec_t × int64) unit ((
+          offset_38,
+          @cast _ uint64 _ (offset_38)
+        ))
+      | None => @Err (contract_state_hacspec_t × int64) unit (tt)
+      end) else (match pub_int64_checked_abs (delta_37) with
+      | Some b_39 => match pub_uint32_checked_sub (current_position_31) (
+        @cast _ uint32 _ (b_39)) with
+      | Some offset_40 => @Ok (contract_state_hacspec_t × int64) unit ((
+          offset_40,
+          @cast _ uint64 _ (offset_40)
+        ))
+      | None => @Err (contract_state_hacspec_t × int64) unit (tt)
+      end
+      | None => @Err (contract_state_hacspec_t × int64) unit (tt)
+      end))
+  end.
+
+Definition contract_state_impl_read_read
+  (current_position_41 : contract_state_hacspec_t)
+  (buf_42 : public_byte_seq)
+  : (contract_state_hacspec_t × uint_size) :=
+  let '(buf_43, num_read_44) :=
+    load_state_hacspec (buf_42) (current_position_41) in 
+  ((current_position_41) .+ (num_read_44), @cast _ uint32 _ (num_read_44)).
+
+Definition contract_state_impl_read_read_u64
+  (current_position_45 : contract_state_hacspec_t)
+  : (contract_state_hacspec_t × int64) :=
+  let buf_46 : seq int8 :=
+    seq_new_ (default) (usize 8) in 
+  let '(buf_47, num_read_48) :=
+    load_state_hacspec (buf_46) (current_position_45) in 
+  (
+    (current_position_45) .+ (num_read_48),
+    u64_from_le_bytes (array_from_seq (8) (buf_47))
+  ).
+
+Definition contract_state_impl_read_read_u32
+  (current_position_49 : contract_state_hacspec_t)
+  : (contract_state_hacspec_t × int32) :=
+  let buf_50 : seq int8 :=
+    seq_new_ (default) (usize 4) in 
+  let '(buf_51, num_read_52) :=
+    load_state_hacspec (buf_50) (current_position_49) in 
+  (
+    (current_position_49) .+ (num_read_52),
+    u32_from_le_bytes (array_from_seq (4) (buf_51))
+  ).
+
+Definition contract_state_impl_read_read_u8
+  (current_position_53 : contract_state_hacspec_t)
+  : (contract_state_hacspec_t × int8) :=
+  let buf_54 : seq int8 :=
+    seq_new_ (default) (usize 1) in 
+  let '(buf_55, num_read_56) :=
+    load_state_hacspec (buf_54) (current_position_53) in 
+  ((current_position_53) .+ (num_read_56), seq_index (buf_55) (usize 0)).
+
+Definition contract_state_impl_write
+  (current_position_57 : contract_state_hacspec_t)
+  (buf_58 : public_byte_seq)
+  : (result (contract_state_hacspec_t × uint_size) unit) :=
+  ifbnd option_is_none (pub_uint32_checked_add (current_position_57) (pub_u32 (
+        seq_len (buf_58)))) : bool
+  thenbnd (bind (@Err (contract_state_hacspec_t × uint_size) unit (tt)) (
+      fun _ => Ok (tt)))
+  else (tt) >> (fun 'tt =>
+  let '(buf_59, num_bytes_60) :=
+    write_state_hacspec (buf_58) (current_position_57) in 
+  @Ok (contract_state_hacspec_t × uint_size) unit ((
+      (current_position_57) .+ (num_bytes_60),
+      @cast _ uint32 _ (num_bytes_60)
+    ))).
+
+Definition has_contract_state_impl_for_contract_state_open
+  
+  : contract_state_hacspec_t :=
+  @repr WORDSIZE32 0.
+
+Definition has_contract_state_impl_for_contract_state_reserve
+  (contract_state_61 : contract_state_hacspec_t)
+  (len_62 : int32)
+  : bool :=
+  let cur_size_63 : int32 :=
+    state_size_hacspec  in 
+  (if ((cur_size_63) <.? (len_62)):bool then ((resize_state_hacspec (
+          len_62)) =.? (@repr WORDSIZE32 1)) else (true)).
+
+Definition has_contract_state_impl_for_contract_state_truncate
+  (current_position_64 : contract_state_hacspec_t)
+  (cur_size_65 : int32)
+  (new_size_66 : int32)
+  : contract_state_hacspec_t :=
+  let 'tt :=
+    if (cur_size_65) >.? (new_size_66):bool then (let _ : int32 :=
+        resize_state_hacspec (new_size_66) in 
+      tt) else (tt) in 
+  (if ((new_size_66) <.? (current_position_64)):bool then (new_size_66) else (
+      current_position_64)).
+
+Notation "'parameter_hacspec_t'" := (int32) : hacspec_scope.
+
+Definition read_impl_for_parameter_read
+  (current_position_67 : parameter_hacspec_t)
+  (buf_68 : public_byte_seq)
+  : (parameter_hacspec_t × uint_size) :=
+  let '(buf_69, num_read_70) :=
+    get_parameter_section_hacspec (buf_68) (current_position_67) in 
+  ((current_position_67) .+ (num_read_70), @cast _ uint32 _ (num_read_70)).
+
+Notation "'attributes_cursor_hacspec_t'" := ((int32 × int16)) : hacspec_scope.
+
+Definition has_policy_impl_for_policy_attributes_cursor_next_item
+  (policy_attribute_items_71 : attributes_cursor_hacspec_t)
+  (buf_72 : public_byte_seq)
+  : (option (attributes_cursor_hacspec_t × (int8 × int8))) :=
+  let '(current_position_73, remaining_items_74) :=
+    policy_attribute_items_71 in 
+  ifbnd (remaining_items_74) =.? (@repr WORDSIZE16 0) : bool
+  thenbnd (bind (@None (attributes_cursor_hacspec_t × (int8 × int8))) (
+      fun _ => Some (tt)))
+  else (tt) >> (fun 'tt =>
+  let '(tag_value_len_75, num_read_76) :=
+    get_policy_section_hacspec (seq_new_ (default) (usize 2)) (
+      current_position_73) in 
+  let current_position_73 :=
+    (current_position_73) .+ (num_read_76) in 
+  ifbnd (seq_index (tag_value_len_75) (usize 1)) >.? (@repr WORDSIZE8 31) : bool
+  thenbnd (bind (@None (attributes_cursor_hacspec_t × (int8 × int8))) (
+      fun _ => Some (tt)))
+  else (tt) >> (fun 'tt =>
+  let '(buf_77, num_read_78) :=
+    get_policy_section_hacspec (buf_72) (current_position_73) in 
+  let current_position_73 :=
+    (current_position_73) .+ (num_read_78) in 
+  let remaining_items_74 :=
+    (remaining_items_74) .- (@repr WORDSIZE16 1) in 
+  @Some (attributes_cursor_hacspec_t × (int8 × int8)) ((
+      (current_position_73, remaining_items_74),
+      (
+        seq_index (tag_value_len_75) (usize 0),
+        seq_index (tag_value_len_75) (usize 1)
+      )
+    )))).
+
+Notation "'policies_iterator_hacspec_t'" := ((int32 × int16)) : hacspec_scope.
+
+Notation "'policy_attributes_cursor_hacspec_t'" := ((
+  int32 ×
+  int64 ×
+  int64 ×
+  attributes_cursor_hacspec_t
+)) : hacspec_scope.
+
+Definition iterator_impl_for_policies_iterator_next
+  (policies_iterator_79 : policies_iterator_hacspec_t)
+  : (option (policies_iterator_hacspec_t × policy_attributes_cursor_hacspec_t
+    )) :=
+  let '(pos_80, remaining_items_81) :=
+    policies_iterator_79 in 
+  ifbnd (remaining_items_81) =.? (@repr WORDSIZE16 0) : bool
+  thenbnd (bind (@None (
+        policies_iterator_hacspec_t ×
+        policy_attributes_cursor_hacspec_t
+      )) (fun _ => Some (tt)))
+  else (tt) >> (fun 'tt =>
+  let '(buf_82, _) :=
+    get_policy_section_hacspec (seq_new_ (default) (((((usize 2) + (
+                usize 4)) + (usize 8)) + (usize 8)) + (usize 2))) (pos_80) in 
+  let skip_part_83 : public_byte_seq :=
+    seq_slice_range (buf_82) ((usize 0, usize 2)) in 
+  let ip_part_84 : public_byte_seq :=
+    seq_slice_range (buf_82) ((usize 2, (usize 2) + (usize 4))) in 
+  let created_at_part_85 : public_byte_seq :=
+    seq_slice_range (buf_82) ((
+        (usize 2) + (usize 4),
+        ((usize 2) + (usize 4)) + (usize 8)
+      )) in 
+  let valid_to_part_86 : public_byte_seq :=
+    seq_slice_range (buf_82) ((
+        ((usize 2) + (usize 4)) + (usize 8),
+        (((usize 2) + (usize 4)) + (usize 8)) + (usize 8)
+      )) in 
+  let len_part_87 : public_byte_seq :=
+    seq_slice_range (buf_82) ((
+        (((usize 2) + (usize 4)) + (usize 8)) + (usize 8),
+        ((((usize 2) + (usize 4)) + (usize 8)) + (usize 8)) + (usize 2)
+      )) in 
+  let identity_provider_88 : int32 :=
+    u32_from_le_bytes (array_from_seq (4) (ip_part_84)) in 
+  let created_at_89 : int64 :=
+    u64_from_le_bytes (array_from_seq (8) (created_at_part_85)) in 
+  let valid_to_90 : int64 :=
+    u64_from_le_bytes (array_from_seq (8) (valid_to_part_86)) in 
+  let remaining_items_91 : int16 :=
+    u16_from_le_bytes (array_from_seq (2) (len_part_87)) in 
+  let attributes_start_92 : int32 :=
+    (((((pos_80) .+ (@repr WORDSIZE32 2)) .+ (@repr WORDSIZE32 4)) .+ (
+          @repr WORDSIZE32 8)) .+ (@repr WORDSIZE32 8)) .+ (
+      @repr WORDSIZE32 2) in 
+  let pos_80 :=
+    ((pos_80) .+ (@cast _ uint32 _ (u16_from_le_bytes (array_from_seq (2) (
+              skip_part_83))))) .+ (@repr WORDSIZE32 2) in 
+  let remaining_items_91 :=
+    (remaining_items_91) .- (@repr WORDSIZE16 1) in 
+  @Some (policies_iterator_hacspec_t × policy_attributes_cursor_hacspec_t) ((
+      (pos_80, remaining_items_91),
+      (
+        identity_provider_88,
+        created_at_89,
+        valid_to_90,
+        (attributes_start_92, remaining_items_91)
+      )
+    ))).
+
 Require Import Hacspec.Concordium_Types.
 
 Require Import Hacspec.Concordium_Traits.
